tests/Add.bpl
@@ -1,0 +1,139 @@
+// ---------------------------------------------------------------
+// -- Types and global variables ---------------------------------
+// ---------------------------------------------------------------
+type Chan a;
+type Actor;
+type CType = <a>[Chan a]int;
+type MType = <a>[Chan a][int]a;
+type State;
+
+var M: MType;
+var C: CType;
+var R: CType; 
+var N: CType;
+var C#init: CType;
+var St: [Actor]State;
+
+const unique this#: Actor;
+
+type List a = [int]a;
+var AT#intlst: List int;
+
+
+// ---------------------------------------------------------------
+// -- End of prelude ---------------------------------------------
+// ---------------------------------------------------------------
+
+procedure Add#anon$0#0()
+  modifies C, R, M, St;
+{
+  var IV#in1#i: int;
+  var IV#in2#j: int;
+  assume true;
+}
+procedure Net#init#1()
+  modifies C, R, M, St;
+{
+  assume C[Net#a] == 0;
+  assume R[Net#a] == 0;
+  assume C[Net#b] == 0;
+  assume R[Net#b] == 0;
+  assume C[Net#c] == 0;
+  assume R[Net#c] == 0;
+}
+const unique Net#add: Actor;
+const unique Net#a: Chan (int);
+const unique Net#b: Chan (int);
+const unique Net#c: Chan (int);
+procedure Net#anon$1#entry#2()
+  modifies C, R, M, St;
+{
+  var ActionPH#y: int;
+  assume C#init[Net#a] == 1;
+  assume C#init[Net#b] == 1;
+  assume C#init[Net#c] == 0;
+  assume R[Net#a] == 0;
+  assume R[Net#b] == 0;
+  assume R[Net#c] == 0;
+  assume C#init == C;
+  assert {:msg "  Channel invariant might not hold on action entry (generated #0)"} 0 <= R[Net#a];
+  assert {:msg "  Channel invariant might not hold on action entry (generated #1)"} 0 <= C[Net#a];
+  assert {:msg "  Channel invariant might not hold on action entry (generated #2)"} (R[Net#a] + C[Net#a]) == C#init[Net#a];
+  assert {:msg "  Channel invariant might not hold on action entry (generated #3)"} 0 <= R[Net#b];
+  assert {:msg "  Channel invariant might not hold on action entry (generated #4)"} 0 <= C[Net#b];
+  assert {:msg "  Channel invariant might not hold on action entry (generated #5)"} (R[Net#b] + C[Net#b]) == C#init[Net#b];
+  assert {:msg "  Channel invariant might not hold on action entry (generated #6)"} 0 <= R[Net#c];
+  assert {:msg "  Channel invariant might not hold on action entry (generated #7)"} 0 <= C[Net#c];
+  assert {:msg "  Channel invariant might not hold on action entry (generated #8)"} R[Net#c] == 0;
+  assert {:msg "  12.3: Channel invariant might not hold on action entry"} R[Net#a] == (R[Net#c] + C[Net#c]);
+  assert {:msg "  13.3: Channel invariant might not hold on action entry"} R[Net#b] == (R[Net#c] + C[Net#c]);
+}
+procedure Net#anon$1#Add#anon$0#3()
+  modifies C, R, M, St;
+{
+  var St#next: State;
+  var in1#i: int;
+  var in2#j: int;
+  assume C#init[Net#a] == 1;
+  assume C#init[Net#b] == 1;
+  assume C#init[Net#c] == 0;
+  assume 0 <= R[Net#a];
+  assume 0 <= C[Net#a];
+  assume (R[Net#a] + C[Net#a]) == C#init[Net#a];
+  assume 0 <= R[Net#b];
+  assume 0 <= C[Net#b];
+  assume (R[Net#b] + C[Net#b]) == C#init[Net#b];
+  assume 0 <= R[Net#c];
+  assume 0 <= C[Net#c];
+  assume R[Net#c] == 0;
+  assume R[Net#a] == (R[Net#c] + C[Net#c]);
+  assume R[Net#b] == (R[Net#c] + C[Net#c]);
+  assume true;
+  assume (1 <= C[Net#a]) && (1 <= C[Net#b]);
+  in1#i := M[Net#a][R[Net#a]];
+  R[Net#a] := R[Net#a] + 1;
+  C[Net#a] := C[Net#a] - 1;
+  in2#j := M[Net#b][R[Net#b]];
+  R[Net#b] := R[Net#b] + 1;
+  C[Net#b] := C[Net#b] - 1;
+  M[Net#c][R[Net#c] + C[Net#c]] := in1#i + in2#j;
+  C[Net#c] := C[Net#c] + 1;
+  assert {:msg "  Sub-actor action at 3.3 might not preserve the channel invariant (generated #9)"} 0 <= R[Net#a];
+  assert {:msg "  Sub-actor action at 3.3 might not preserve the channel invariant (generated #10)"} 0 <= C[Net#a];
+  assert {:msg "  Sub-actor action at 3.3 might not preserve the channel invariant (generated #11)"} (R[Net#a] + C[Net#a]) == C#init[Net#a];
+  assert {:msg "  Sub-actor action at 3.3 might not preserve the channel invariant (generated #12)"} 0 <= R[Net#b];
+  assert {:msg "  Sub-actor action at 3.3 might not preserve the channel invariant (generated #13)"} 0 <= C[Net#b];
+  assert {:msg "  Sub-actor action at 3.3 might not preserve the channel invariant (generated #14)"} (R[Net#b] + C[Net#b]) == C#init[Net#b];
+  assert {:msg "  Sub-actor action at 3.3 might not preserve the channel invariant (generated #15)"} 0 <= R[Net#c];
+  assert {:msg "  Sub-actor action at 3.3 might not preserve the channel invariant (generated #16)"} 0 <= C[Net#c];
+  assert {:msg "  Sub-actor action at 3.3 might not preserve the channel invariant (generated #17)"} R[Net#c] == 0;
+  assert {:msg "  12.3: Sub-actor action at 3.3 might not preserve the channel invariant"} R[Net#a] == (R[Net#c] + C[Net#c]);
+  assert {:msg "  13.3: Sub-actor action at 3.3 might not preserve the channel invariant"} R[Net#b] == (R[Net#c] + C[Net#c]);
+}
+procedure Net#anon$1#exit#4()
+  modifies C, R, M, St;
+{
+  var ActionPH#y: int;
+  assume C#init[Net#a] == 1;
+  assume C#init[Net#b] == 1;
+  assume C#init[Net#c] == 0;
+  assume 0 <= R[Net#a];
+  assume 0 <= C[Net#a];
+  assume (R[Net#a] + C[Net#a]) == C#init[Net#a];
+  assume 0 <= R[Net#b];
+  assume 0 <= C[Net#b];
+  assume (R[Net#b] + C[Net#b]) == C#init[Net#b];
+  assume 0 <= R[Net#c];
+  assume 0 <= C[Net#c];
+  assume R[Net#c] == 0;
+  assume R[Net#a] == (R[Net#c] + C[Net#c]);
+  assume R[Net#b] == (R[Net#c] + C[Net#c]);
+  assume !((1 <= C[Net#a]) && (1 <= C[Net#b]));
+  assert {:msg "  8.3: The network might leave unread tokens on channel a"} C[Net#a] == 0;
+  assert {:msg "  8.3: The network might leave unread tokens on channel b"} C[Net#b] == 0;
+  assert {:msg "  8.3: The network might not produce the specified number of tokens on output out"} C[Net#c] == 1;
+  ActionPH#y := M[Net#c][0];
+  assert {:msg "  9.13: Network action postcondition might not hold"} ActionPH#y == (M[Net#a][0] + M[Net#b][0]);
+  R[Net#c] := R[Net#c] + C[Net#c];
+  C[Net#c] := 0;
+}
