tests/State.bpl
@@ -1,0 +1,44 @@
+// ---------------------------------------------------------------
+// -- Types and global variables ---------------------------------
+// ---------------------------------------------------------------
+type Chan a;
+type Actor;
+type CType = <a>[Chan a]int;
+type MType = <a>[Chan a][int]a;
+type State;
+
+var M: MType;
+var C: CType;
+var R: CType; 
+var N: CType;
+var C#init: CType;
+var St: [Actor]State;
+
+const unique this#: Actor;
+
+type List a = [int]a;
+var AT#intlst: List int;
+
+
+// ---------------------------------------------------------------
+// -- End of prelude ---------------------------------------------
+// ---------------------------------------------------------------
+
+procedure Sum#anon$0#0()
+  modifies C, R, M, St;
+{
+  var sum: int;
+  assume 0 <= sum;
+  sum := 0;
+  assert {:msg "  6.13: Action at 8.3 might not preserve invariant"} 0 <= sum;
+}
+procedure Sum#anon$1#1()
+  modifies C, R, M, St;
+{
+  var sum: int;
+  var IV#in1#i: int;
+  assume 0 <= sum;
+  assume 0 <= IV#in1#i;
+  sum := sum + IV#in1#i;
+  assert {:msg "  6.13: Action at 13.3 might not preserve invariant"} 0 <= sum;
+}
